unifying labels and operations

examples/layeredeffects/LatticeAlg.fst
@@ -5,10 +5,9 @@ module LatticeAlg
 open FStar.Tactics
 open FStar.List.Tot
 open FStar.Universe
-
 module WF = FStar.WellFounded
+module L = Lattice
 
-// GM: Force a type equality by SMT
 let coerce #a #b (x:a{a == b}) : b = x
 
 let unreachable (#a:Type u#aa) () : Pure a (requires False) (ensures (fun _ -> False)) =
@@ -16,103 +15,57 @@ let unreachable (#a:Type u#aa) () : Pure a (requires False) (ensures (fun _ -> F
 
 type state = int
 
-type eff_label =
-  | RD
-  | WR
-  | EXN
+type op =
+  | Read
+  | Write
+  | Raise
+  | Other of int
+
+assume val other_inp : int -> Type
+let op_inp : op -> Type =
+ function
+ | Read -> unit
+ | Write -> state
+ | Raise -> exn
+ | Other i -> other_inp i
+
+assume val other_out : int -> Type
+let op_out : op -> Type =
+ function
+ | Read -> state
+ | Write -> unit
+ | Raise -> c_False
+ | Other i -> other_inp i
 
 noeq
-type action : Type0 -> Type0 -> Type u#1 =
-  | Read : action unit state
-  | Write : action state unit
-  | Raise : action exn c_False
-
-noeq
-type repr0 (a:Type u#aa) : Type u#(max 1 aa) =
+type repr0 (a:Type u#aa) : Type u#aa =
   | Return : a -> repr0 a
-  | Act    : #i:_ -> #o:_ -> act:(action i o) -> i -> k:(o -> repr0 a) -> repr0 a
+  | Act    : op:op -> i:(op_inp op) -> k:(op_out op -> repr0 a) -> repr0 a
 
-type annot = eff_label -> bool
-
-let interp (l : list eff_label) : annot =
-  fun lab -> mem lab l
-
-let label_of #ii #oo (a:action ii oo) : eff_label =
- match a with
- | Read -> RD
- | Write -> WR
- | Raise -> EXN
-
-let label_ii (l:eff_label) : Type =
- match l with
- | RD -> unit
- | WR -> state
- | EXN -> exn
-
-let label_oo (l:eff_label) : Type =
- match l with
- | RD -> state
- | WR -> unit
- | EXN -> c_False
-
-let action_of (l:eff_label) : action (label_ii l) (label_oo l) =
-  match l with
-  | RD ->  Read
-  | WR ->  Write
-  | EXN -> Raise
-
-let iso1 (l:eff_label)
-  : Lemma (label_of (action_of l) == l)
-          [SMTPat (action_of l)]
-  = ()
-  
-let iso2 (a:action 'i 'o)
-  : Lemma (action_of (label_of a) == a)
-          [SMTPat (label_of a)]
-  = ()
-
-let abides_act #i #o (ann:annot) (a : action i o) : prop =
-  ann (label_of a) == true
-
-let rec abides #a (ann:annot) (f : repr0 a) : prop =
+let rec abides #a (labs:list op) (f : repr0 a) : prop =
   begin match f with
   | Act a i k ->
-    abides_act ann a /\ (forall o. (FStar.WellFounded.axiom1 k o; abides ann (k o)))
+    mem a labs /\ (forall o. (FStar.WellFounded.axiom1 k o; abides labs (k o)))
   | Return _ -> True
   end
 
 type repr (a:Type u#aa)
-          (labs : list u#0 eff_label) // #2074
-  : Type u#(max 1 aa)
+          (labs : list u#0 op)
+  : Type u#aa
   =
-  r:(repr0 a){abides (interp labs) r}
+  r:(repr0 a){abides labs r}
 
-let rec interp_at (l1 l2 : list eff_label) (l : eff_label)
-  : Lemma (interp (l1@l2) l == (interp l1 l || interp l2 l))
-          [SMTPat (interp (l1@l2) l)]
+let rec interp_at (l1 l2 : list op) (l : op)
+  : Lemma (mem l (l1@l2) == (mem l l1 || mem l l2))
+          [SMTPat (mem l (l1@l2))]
   = match l1 with
     | [] -> ()
     | _::l1 -> interp_at l1 l2 l
 
-let sublist (l1 l2 : list eff_label) =
-  forall x. mem x l1 ==> mem x l2
-
-let sublist_refl
-  (l : list eff_label)
-  : Lemma (sublist l l)
-          [SMTPat (sublist l l)]
-  = ()
-
-let rec interp_sublist (l1 l2 : list eff_label) (l : eff_label)
-  : Lemma (requires (sublist l1 l2))
-          (ensures (interp l1 l ==> interp l2 l))
-          [SMTPat (interp l1 l); SMTPat (sublist l1 l2)]
-  = match l1 with
-    | [] -> ()
-    | _::l1 -> interp_sublist l1 l2 l
+let sublist (l1 l2 : list op) = forall x. mem x l1 ==> mem x l2
 
 let rec sublist_at
-  (l1 l2 : list eff_label)
+  (l1 l2 : list op)
   : Lemma (sublist l1 (l1@l2) /\ sublist l2 (l1@l2))
           [SMTPatOr [[SMTPat (sublist l1 (l1@l2))];
                      [SMTPat (sublist l2 (l1@l2))]]]
@@ -120,38 +73,51 @@ let rec sublist_at
     | [] -> ()
     | _::l1 -> sublist_at l1 l2
 
-let rec abides_sublist_nopat #a (l1 l2 : list eff_label) (c : repr0 a)
-  : Lemma (requires (abides (interp l1) c) /\ sublist l1 l2)
-          (ensures (abides (interp l2) c))
+let sublist_at_self
+  (l : list op)
+  : Lemma (sublist l (l@l))
+          [SMTPat (sublist l (l@l))]
+  = ()
+  
+let rec abides_sublist_nopat #a (l1 l2 : list op) (c : repr0 a)
+  : Lemma (requires (abides l1 c) /\ sublist l1 l2)
+          (ensures (abides l2) c)
   = match c with
     | Return _ -> ()
     | Act a i k ->
-      let sub o : Lemma (abides (interp l2) (k o)) =
+      let sub o : Lemma (abides l2 (k o)) =
         FStar.WellFounded.axiom1 k o;
         abides_sublist_nopat l1 l2 (k o)
       in
       Classical.forall_intro sub
 
-let abides_sublist #a (l1 l2 : list eff_label) (c : repr0 a)
-  : Lemma (requires (abides (interp l1) c) /\ sublist l1 l2)
-          (ensures (abides (interp l2) c))
-          [SMTPat (abides (interp l2) c); SMTPat (sublist l1 l2)]
+let abides_sublist #a (l1 l2 : list op) (c : repr0 a)
+  : Lemma (requires (abides l1 c) /\ sublist l1 l2)
+          (ensures (abides l2 c))
+          [SMTPat (abides l2 c); SMTPat (sublist l1 l2)]
   = abides_sublist_nopat l1 l2 c
+  
+let abides_at_self #a
+  (l : list op)
+  (c : repr0 a)
+  : Lemma (abides (l@l) c <==>  abides l c)
+          [SMTPat (abides (l@l) c)]
+  = (* Trigger some patterns *)
+    assert (sublist l (l@l));
+    assert (sublist (l@l) l)
 
-let abides_app #a (l1 l2 : list eff_label) (c : repr0 a)
-  : Lemma (requires (abides (interp l1) c \/ abides (interp l2) c))
-          (ensures (abides (interp (l1@l2)) c))
-          [SMTPat (abides (interp (l1@l2)) c)]
-  = Classical.move_requires (abides_sublist_nopat l1 (l1@l2)) c;
-    Classical.move_requires (abides_sublist_nopat l2 (l1@l2)) c
+let abides_app #a (l1 l2 : list op) (c : repr0 a)
+  : Lemma (requires (abides l1 c \/ abides l2 c))
+          (ensures (abides (l1@l2) c))
+          [SMTPat (abides (l1@l2) c)]
+  = sublist_at l1 l2
 
 let return (a:Type) (x:a)
   : repr a []
-  =
-  Return x
+  = Return x
 
 let rec bind (a b : Type)
-  (labs1 labs2 : list eff_label)
+  (labs1 labs2 : list op)
   (c : repr a labs1)
   (f : (x:a -> repr b labs2))
   : Tot (repr b (labs1@labs2))
@@ -165,7 +131,7 @@ let rec bind (a b : Type)
       Act act i k'
 
 let subcomp (a:Type)
-  (labs1 labs2 : list eff_label)
+  (labs1 labs2 : list op)
   (f : repr a labs1)
   : Pure (repr a labs2)
          (requires (sublist labs1 labs2))
@@ -174,21 +140,21 @@ let subcomp (a:Type)
 
 let if_then_else
   (a : Type)
-  (labs1 labs2 : list eff_label)
+  (labs1 labs2 : list op)
   (f : repr a labs1)
   (g : repr a labs2)
   (p : bool)
   : Type
   = repr a (labs1@labs2)
 
-let _get () : repr int [RD] = Act Read () Return
+let _get () : repr int [Read] = Act Read () Return
 
 [@@allow_informative_binders]
 total // need this for catch!!
 reifiable
 reflectable
 layered_effect {
-  EFF : a:Type -> list eff_label  -> Effect
+  EFF : a:Type -> list op  -> Effect
   with
   repr         = repr;
   return       = return;
@@ -197,7 +163,7 @@ layered_effect {
   if_then_else = if_then_else
 }
 
-let get () : EFF int [RD] =
+let get () : EFF int [Read] =
   EFF?.reflect (_get ())
 
 unfold
@@ -219,29 +185,24 @@ let lift_pure_eff
 
 sub_effect PURE ~> EFF = lift_pure_eff
 
-let put (s:state) : EFF unit [WR] =
+let put (s:state) : EFF unit [Write] =
   EFF?.reflect (Act Write s Return)
 
-let raise #a (e:exn) : EFF a [EXN] =
+let raise #a (e:exn) : EFF a [Raise] =
   EFF?.reflect (Act Raise e Return)
 
 exception Failure of string
 
-let test0 (x y : int) : EFF int [RD; EXN] =
+let test0 (x y : int) : EFF int [Read; Raise] =
   let z = get () in
   if z < 0 then raise (Failure "error");
   x + y + z
 
-let test1 (x y : int) : EFF int [EXN; RD; WR] =
+let test1 (x y : int) : EFF int [Raise; Read; Write] =
   let z = get () in
   if x + z > 0
   then raise (Failure "asd")
   else (put 42; y - z)
-
-let sublist_at_self (l1 : list eff_label)
-  : Lemma (sublist (l1@l1) l1)
-          [SMTPat (l1@l1)]
-  = Classical.forall_intro (List.Tot.Properties.append_mem l1 l1)
 
 let labpoly #labs (f g : unit -> EFF int labs) : EFF int labs =
   f () + g ()
@@ -258,8 +219,8 @@ let labpoly #labs (f g : unit -> EFF int labs) : EFF int labs =
 // Called from file "src/ocaml-output/FStar_TypeChecker_TcTerm.ml", line 2048, characters 30-68
 // Called from file "src/basic/ml/FStar_Util.ml", line 24, characters 14-18
 // ....
-let rec catch0 #a #labs (t1 : repr a (EXN::labs))
-                    (t2 : repr a labs)
+let rec catch0 #a #labs (t1 : repr a (Raise::labs))
+                        (t2 : repr a labs)
   : repr a labs
   = match t1 with
     | Act Raise e _ -> t2
@@ -273,7 +234,7 @@ let rec catch0 #a #labs (t1 : repr a (EXN::labs))
 
 (* no rollback *)
 let catch #a #labs
-  (f : unit -> EFF a (EXN::labs))
+  (f : unit -> EFF a (Raise::labs))
   (g : unit -> EFF a labs)
   : EFF a labs
 =
@@ -281,7 +242,7 @@ let catch #a #labs
    catch0 (reify (f ())) (reify (g ()))
  end
 
-let rec _catchST #a #labs (t1 : repr a (RD::WR::labs)) (s0:state) : repr (a & int) labs =
+let rec _catchST #a #labs (t1 : repr a (Read::Write::labs)) (s0:state) : repr (a & int) labs =
   match t1 with
   | Return v -> Return (v, s0)
   | Act Write s k -> WF.axiom1 k (); _catchST (k ()) s
@@ -294,7 +255,7 @@ let rec _catchST #a #labs (t1 : repr a (RD::WR::labs)) (s0:state) : repr (a & in
      Act act i k'
 
 let catchST #a #labs
-  (f : unit -> EFF a (RD::WR::labs))
+  (f : unit -> EFF a (Read::Write::labs))
   (s0 : state)
   : EFF (a & state) labs
 =
@@ -304,10 +265,10 @@ let catchST #a #labs
 
 let g #labs () : EFF int labs = 42  //AR: 07/03: had to hoist after removing smt_reifiablep
 
-let test_catch #labs (f : unit -> EFF int [EXN;WR]) : EFF int [WR] =
+let test_catch #labs (f : unit -> EFF int [Raise;Write]) : EFF int [Write] =
   catch f g
 
-let test_catch2 (f : unit -> EFF int [EXN;EXN;WR]) : EFF int [EXN;WR] =
+let test_catch2 (f : unit -> EFF int [Raise;Raise;Write]) : EFF int [Raise;Write] =
   catch f g
 
 let interp_pure_tree #a (t : repr a []) : Tot a =
@@ -316,16 +277,16 @@ let interp_pure_tree #a (t : repr a []) : Tot a =
 
 let interp_pure #a (f : unit -> EFF a []) : Tot a = interp_pure_tree (reify (f ()))
 
-let rec interp_rd_tree #a (t : repr a [RD]) (s:state) : Tot a =
+let rec interp_rd_tree #a (t : repr a [Read]) (s:state) : Tot a =
   match t with
   | Return x -> x
   | Act Read _ k ->
     FStar.WellFounded.axiom1 k s;
     interp_rd_tree (k s) s
 
-let interp_rd #a (f : unit -> EFF a [RD]) (s:state) : Tot a = interp_rd_tree (reify (f ())) s
+let interp_rd #a (f : unit -> EFF a [Read]) (s:state) : Tot a = interp_rd_tree (reify (f ())) s
 
-let rec interp_rdwr_tree #a (t : repr a [RD;WR]) (s:state) : Tot (a & state) =
+let rec interp_rdwr_tree #a (t : repr a [Read;Write]) (s:state) : Tot (a & state) =
   match t with
   | Return x -> (x, s)
   | Act Read _ k ->
@@ -335,9 +296,9 @@ let rec interp_rdwr_tree #a (t : repr a [RD;WR]) (s:state) : Tot (a & state) =
     FStar.WellFounded.axiom1 k ();
     interp_rdwr_tree (k ()) s
 
-let interp_rdwr #a (f : unit -> EFF a [RD;WR]) (s:state) : Tot (a & state) = interp_rdwr_tree (reify (f ())) s
+let interp_rdwr #a (f : unit -> EFF a [Read;Write]) (s:state) : Tot (a & state) = interp_rdwr_tree (reify (f ())) s
 
-let rec interp_rdexn_tree #a (t : repr a [RD;EXN]) (s:state) : Tot (option a) =
+let rec interp_rdexn_tree #a (t : repr a [Read;Raise]) (s:state) : Tot (option a) =
   match t with
   | Return x -> Some x
   | Act Read _ k ->
@@ -346,9 +307,9 @@ let rec interp_rdexn_tree #a (t : repr a [RD;EXN]) (s:state) : Tot (option a) =
   | Act Raise e k ->
     None
 
-let interp_rdexn #a (f : unit -> EFF a [RD;EXN]) (s:state) : Tot (option a) = interp_rdexn_tree (reify (f ())) s
+let interp_rdexn #a (f : unit -> EFF a [Read;Raise]) (s:state) : Tot (option a) = interp_rdexn_tree (reify (f ())) s
 
-let rec interp_all_tree #a (t : repr a [RD;WR;EXN]) (s:state) : Tot (option a & state) =
+let rec interp_all_tree #a (t : repr a [Read;Write;Raise]) (s:state) : Tot (option a & state) =
   match t with
   | Return x -> (Some x, s)
   | Act Read _ k ->
@@ -360,7 +321,7 @@ let rec interp_all_tree #a (t : repr a [RD;WR;EXN]) (s:state) : Tot (option a & 
   | Act Raise e k ->
     (None, s)
 
-let interp_all #a (f : unit -> EFF a [RD;WR;EXN]) (s:state) : Tot (option a & state) = interp_all_tree (reify (f ())) s
+let interp_all #a (f : unit -> EFF a [Read;Write;Raise]) (s:state) : Tot (option a & state) = interp_all_tree (reify (f ())) s
 
 //let action_input (a:action 'i 'o) = 'i
 //let action_output (a:action 'i 'o) = 'o
@@ -378,8 +339,8 @@ let interp_all #a (f : unit -> EFF a [RD;WR;EXN]) (s:state) : Tot (option a & st
 //let dpi33 (#a:Type) (#b:a->Type) (#c:(x:a->b x->Type)) (t : (x:a & y:b x & c x y)) : c (dpi31 t) (dpi32 t) =
 //  let (| x, y, z |) = t in z
 
-let handler_ty_l (l:eff_label) (b:Type) (labs:list eff_label) =
-  label_ii l -> (label_oo l -> repr b labs) -> repr b labs
+let handler_ty_l (o:op) (b:Type) (labs:list op) =
+  op_inp o -> (op_out o -> repr b labs) -> repr b labs
 
   //handler_ty (dpi33 (action_of l)) b labs
   //F* complains this is not a function
@@ -389,16 +350,16 @@ let handler_ty_l (l:eff_label) (b:Type) (labs:list eff_label) =
 (* A generic handler for a (single) label l, relies on the fact that
 we can compare actions for equality, or equivalently map them to their
 labels. *)
-val handle (#a #b:_) (#labs:_) (l:eff_label)
-           (f:repr a (l::labs))
-           (h:handler_ty_l l b labs)
+val handle (#a #b:_) (#labs:_) (o:op)
+           (f:repr a (o::labs))
+           (h:handler_ty_l o b labs)
            (v: a -> repr b labs)
            : repr b labs
 let rec handle #a #b #labs l f h v =
   match f with
   | Return x -> v x
   | Act act i k ->
-    if label_of act = l
+    if act = l
     then h i (fun o -> WF.axiom1 k o; handle l (k o) h v)
     else begin
       let k' o : repr b labs =
@@ -409,7 +370,7 @@ let rec handle #a #b #labs l f h v =
     end
 
 (* Easy enough to handle 2 labels at once *)
-val handle2 (#a #b:_) (#labs:_) (l1 l2 :eff_label)
+val handle2 (#a #b:_) (#labs:_) (l1 l2 : op)
            (f:repr a (l1::l2::labs))
            (h1:handler_ty_l l1 b labs)
            (h2:handler_ty_l l2 b labs)
@@ -419,9 +380,9 @@ let rec handle2 #a #b #labs l1 l2 f h1 h2 v =
   match f with
   | Return x -> v x
   | Act act i k ->
-    if label_of act = l1
+    if act = l1
     then h1 i (fun o -> WF.axiom1 k o; handle2 l1 l2 (k o) h1 h2 v)
-    else if label_of act = l2
+    else if act = l2
     then h2 i (fun o -> WF.axiom1 k o; handle2 l1 l2 (k o) h1 h2 v)
     else begin
       let k' o : repr b labs =
@@ -432,9 +393,9 @@ let rec handle2 #a #b #labs l1 l2 f h1 h2 v =
     end
 
 (* All the way *)
-val handle_with (#a #b:_) (#labs0 #labs1 : list eff_label)
+val handle_with (#a #b:_) (#labs0 #labs1 : list op)
            (f:repr a labs0)
-           (h: (l:eff_label{mem l labs0} -> handler_ty_l l b labs1))
+           (h: (l:op{mem l labs0} -> handler_ty_l l b labs1))
            (v : a -> repr b labs1)
            : repr b labs1
 let rec handle_with #a #b #labs0 #labs1 f h v =
@@ -445,20 +406,20 @@ let rec handle_with #a #b #labs0 #labs1 f h v =
         WF.axiom1 k o;
        handle_with #a #b #labs0 #labs1 (k o) h v
     in
-    h (label_of act) i k'
+    h act i k'
 
-let catch0' #a #labs (t1 : repr a (EXN::labs))
+let catch0' #a #labs (t1 : repr a (Raise::labs))
                      (t2 : repr a labs)
   : repr a labs
-  = handle EXN t1 (fun i k -> t2) (fun x -> Return x)
+  = handle Raise t1 (fun i k -> t2) (fun x -> Return x)
 
-let catch0'' #a #labs (t1 : repr a (EXN::labs))
+let catch0'' #a #labs (t1 : repr a (Raise::labs))
                       (t2 : repr a labs)
   : repr a labs
-  = handle_with t1 (function EXN -> (fun i k -> t2)
-                           | act -> (fun i k -> Act (action_of act) i k))
+  = handle_with t1 (function Raise -> (fun i k -> t2)
+                           | act -> (fun i k -> Act act i k))
                    (fun x -> Return x)
-  
+
 let fmap #a #b #labs (f : a -> b) (t : repr a labs) : repr b labs =
   bind _ _ _ labs t (fun x -> Return (f x))
 
@@ -478,30 +439,30 @@ let frompure #a (t : repr a []) : a =
 #set-options "--print_implicits"
 
 let catchST2_emp #a
-  (f : repr a (RD::WR::[]))
+  (f : repr a (Read::Write::[]))
   : repr (state -> a & state) []
   = handle2 #a #(state -> a & state)
             #[]
-            RD WR f
+            Read Write f
             (fun _  k -> Return (fun s -> frompure (k s) s))
             (fun s' k -> Return (fun s -> frompure (k ()) s'))
             (fun x -> Return (fun s -> (x,s)))
 
 (* The mysterious version without annotations *)
-let catchST2 #a #labs (f : repr a (RD::WR::labs))
+let catchST2 #a #labs (f : repr a (Read::Write::labs))
   : repr (state -> repr (a & state) labs) labs
-  = handle2 RD WR f
+  = handle2 Read Write f
             (fun _ k -> Return (fun s -> bind _ _ _ _ (k s)  (fun f -> f s)))
             (fun s k -> Return (fun _ -> bind _ _ _ _ (k ()) (fun f -> f s)))
             (fun x ->   Return (fun s0 -> Return (x, s0)))
 
 (* Fully annotated *)
 let catchST2_sensible #a #labs
-  (f : repr a (RD::WR::labs))
+  (f : repr a (Read::Write::labs))
   : repr (state -> repr (a & state) labs) labs
   = handle2 #a #(state -> repr (a & state) labs)
             #labs
-            RD WR f
+            Read Write f
             (fun _  (k : (state -> repr (state -> repr (a & state) labs) labs)) ->
                        let ff : state -> repr (a & state) labs =
                          fun s0 -> let f : repr (state -> repr (a&state) labs) labs = k s0 in
@@ -512,22 +473,22 @@ let catchST2_sensible #a #labs
             (fun s' k -> bind _ _ _ labs (k ()) (fun f -> Return (fun _ -> f s')))
             (fun x -> Return (fun s0 -> Return (x, s0)))
 
-module L = Lattice
+let baseop = o:op{not (Other? o)}
 
-let trlab = function
-  | RD  -> L.RD
-  | WR  -> L.WR
-  | EXN -> L.EXN
+let trlab : o:baseop -> L.eff_label = function
+  | Read  -> L.RD
+  | Write  -> L.WR
+  | Raise -> L.EXN
 
 let trlab' = function
-  | L.RD  -> RD
-  | L.WR  -> WR
-  | L.EXN -> EXN
+  | L.RD  -> Read
+  | L.WR  -> Write
+  | L.EXN -> Raise
 
 let trlabs  = List.Tot.map trlab
 let trlabs' = List.Tot.map trlab'
 
-let rec lab_corr (l:eff_label) (ls:list eff_label)
+let rec lab_corr (l:baseop) (ls:list baseop)
   : Lemma (mem l ls <==> mem (trlab l) (trlabs ls))
           [SMTPat (mem l ls)] // needed for interp_into_lattice_repr below
   = match ls with
@@ -536,8 +497,25 @@ let rec lab_corr (l:eff_label) (ls:list eff_label)
 
 (* Tied to the particular repr of Lattice.fst *)
 
-let rec interp_into_lattice_repr #a #labs
-  (t : repr a labs)
+(* no datatype subtyping *)
+let fixup : list baseop -> list op = List.Tot.map #baseop #op (fun x -> x)
+
+let rec fixup_corr (l:baseop) (ls:list baseop)
+  : Lemma (mem l (fixup ls) <==> mem l ls)
+          [SMTPat (mem l (fixup ls))]
+  = match ls with
+    | [] -> ()
+    | l1::ls -> fixup_corr l ls
+    
+let rec fixup_no_other (l:op{Other? l}) (ls:list baseop)
+  : Lemma (mem l (fixup ls) <==> False)
+          [SMTPat (mem l (fixup ls))]
+  = match ls with
+    | [] -> ()
+    | l1::ls -> fixup_no_other l ls
+
+let rec interp_into_lattice_repr #a (#labs:list baseop)
+  (t : repr a (fixup labs))
   : L.repr a (trlabs labs)
   = match t with
     | Return x -> L.return _ x
@@ -554,13 +532,15 @@ let rec interp_into_lattice_repr #a #labs
        (fun x -> WF.axiom1 k x;
               interp_into_lattice_repr #a #labs (k x))
 
-let interp_into_lattice #a #labs
-  (f : unit -> EFF a labs)
+let interp_into_lattice #a (#labs:list baseop)
+  (f : unit -> EFF a (fixup labs))
   : Lattice.EFF a (trlabs labs)
   = Lattice.EFF?.reflect (interp_into_lattice_repr (reify (f ())))
 
-let interp_full #a #labs
-  (f : unit -> EFF a labs)
+// This is rather silly: we reflect and then reify. Maybe define interp_into_lattice
+// directly?
+let interp_full #a (#labs:list baseop)
+  (f : unit -> EFF a (fixup labs))
   : Tot (f:(state -> Tot (option a & state)){Lattice.abides f (Lattice.interp (trlabs labs))})
   = reify (interp_into_lattice #a #labs f)
 
@@ -569,20 +549,20 @@ let interp_full #a #labs
 
 type sem0 (a:Type) : Type = state -> Tot (option a & state)
 
-let abides' (f : sem0 'a) (ann:annot) : prop =
-    (ann RD  = false ==> (forall s0 s1. fst (f s0) == fst (f s1)))
-  /\ (ann WR  = false ==> (forall s0. snd (f s0) == s0))
-  /\ (ann EXN = false ==> (forall s0. Some? (fst (f s0))))
+let abides' (f : sem0 'a) (labs:list baseop) : prop =
+    (not (mem Read  labs) ==> (forall s0 s1. fst (f s0) == fst (f s1)))
+  /\ (not (mem Write labs) ==> (forall s0. snd (f s0) == s0))
+  /\ (not (mem Raise labs) ==> (forall s0. Some? (fst (f s0))))
 
-type sem (a:Type) (labs : list eff_label) = r:(sem0 a){abides' r (interp labs)}
+type sem (a:Type) (labs : list baseop) = r:(sem0 a){abides' r labs}
 
-let rec interp_sem #a #labs (t : repr a labs) : sem a labs =
+let rec interp_sem #a (#labs:list baseop) (t : repr a (fixup labs)) : sem a labs =
   match t with
   | Return x -> fun s0 -> (Some x, s0)
   | Act Read _ k ->
     (* Needs this trick for termination. Trying to call axiom1 within
-     * `r` messes up the refinement about RD. *)
-    let k : (s:state -> (r:repr0 a{r << k})) = fun s -> WF.axiom1 k s; k s in
+     * `r` messes up the refinement about Read. *)
+    let k : (s:state -> (r:(repr a (fixup labs)){r << k})) = fun s -> WF.axiom1 k s; k s in
     let r : sem a labs = fun s0 -> interp_sem #a #labs (k s0) s0 in
     r
   | Act Write s k ->
@@ -595,7 +575,7 @@ a fully normalized tree *)
 
 let interp_from_lattice_repr #a #labs
   (t : L.repr a labs)
-  : repr a [RD;EXN;WR] // conservative
+  : repr a [Read;Raise;Write] // conservative
   = Act Read () (fun s0 ->
      let (r, s1) = t s0 in
      match r with
@@ -605,18 +585,18 @@ let interp_from_lattice_repr #a #labs
 
 
 let read_handler (b:Type)
-                 (labs:list eff_label)
+                 (labs:list op)
                  (s0:state)
-   : handler_ty_l RD b labs
+   : handler_ty_l Read b labs
    = fun _ k -> k s0
 
 
 let handle_read (a:Type)
-                (labs:list eff_label)
-                (f:repr a (RD::labs))
-                (h:handler_ty_l RD a labs)
+                (labs:list op)
+                (f:repr a (Read::labs))
+                (h:handler_ty_l Read a labs)
    : repr a labs
-   = handle RD f h (fun x -> Return x)
+   = handle Read f h (fun x -> Return x)
 
 
 let weaken #a #labs l (f:repr a labs) : repr a (l::labs) =
@@ -624,20 +604,20 @@ let weaken #a #labs l (f:repr a labs) : repr a (l::labs) =
   f
 
 let write_handler (a:Type)
-                  (labs:list eff_label)
-  : handler_ty_l WR a labs
-  = fun s k -> handle_read a labs (weaken RD (k())) (read_handler a labs s)
+                  (labs:list op)
+  : handler_ty_l Write a labs
+  = fun s k -> handle_read a labs (weaken Read (k())) (read_handler a labs s)
 
 
 let handle_write (a:Type)
-                (labs:list eff_label)
-                (f:repr a (WR::labs))
+                (labs:list op)
+                (f:repr a (Write::labs))
    : repr a labs
-   = handle WR f (write_handler a labs) (fun x -> Return x)
+   = handle Write f (write_handler a labs) (fun x -> Return x)
 
 let handle_st (a:Type)
-              (labs: list eff_label)
-              (f:repr a (WR::RD::labs))
+              (labs: list op)
+              (f:repr a (Write::Read::labs))
               (s0:state)
    : repr a labs
    = handle_read _ _ (handle_write _ _ f) (fun _ k -> k s0)
